Negationï¼š
$$
-^u_wx=\left\{
\begin{aligned}
&x, &x= 0\\
&2^w - x, &x > 0
\end{aligned}
\right.
$$
$(2^w - x + x) \text{mod} 2^w = 0$ , so $-x = 2^w - x$

Multiplication:
$$
x*^w_wy = (x\cdot y)\text{mod}2^w
$$

### Two's-Complement

$^t_w$. t means two's-complement. for $-2^{w - 1} \le x, y\le2^{w - 1} - 1$
$$
x+^t_wy=\left\{
\begin{aligned}
&x + y - 2^w, & 2^{x - 1} \le x+ y,\ \text{Positive overflow}\\
&x + y, &-2^{w- 1} \le x + y \le 2^{w _ 1} - 1,\ \text{Normal}\\
&x + y + 2 ^w, &x + y < -2^{w - 1}\ \text{Negative overflow}
\end{aligned}
\right.
$$
